
We will use \cite{draft}[Lemma 4.2.11]:

\begin{lemma}
  \label{closed-implies-open-to-or}
  Let $C$ be a closed proposition and $U$ be an open proposition,
  then $C\to U$ is equivalent to $\neg C \vee U$.
\end{lemma}

We will also need:

\begin{lemma}
  \label{commute-open-in-closed-prop}
  Let $C$ be a closed proposition and $U\subseteq C$ open.
  Then there merely is an open proposition $\tilde{U}$ such that $\tilde{U}\cap C = U$.
\end{lemma}

\begin{proof}
  Without loss of generality, assume, $C=\Spec R/(f)$ and $U=D(g)$ with $g:R/(f)$.
  There merely is $\tilde{g}:R$ with $g=\tilde{g}+(f)$.
  By this equality, $D(\tilde{g})\cap C = D(g)$ holds.
\end{proof}
